

---

**第1题**  

$$
\int \frac{x^3}{x+3} dx
$$

解：

$$
\int \frac{x^3}{x+3} dx = \int \left( x^2 - 3x + 9 - \frac{27}{x+3} \right) dx
$$

$$
= \frac{1}{3}x^3 - \frac{3}{2}x^2 + 9x - 27\ln|x+3| + C
$$

---

**第2题**  

$$
\int \frac{2x+3}{x^2+3x-10} dx
$$
解： 

$$
\int \frac{2x+3}{x^2+3x-10} dx = \int \frac{d(x^2+3x-10)}{x^2+3x-10}
$$

$$
= \ln|x^2+3x-10| + C
$$

---

**第3题**  

$$
\int \frac{x+1}{x^2-2x+5} dx
$$
解： 

$$
\int \frac{x+1}{x^2-2x+5} dx = \frac12 \int \frac{2x-2}{x^2-2x+5} dx + 2\int \frac{dx}{(x-1)^2+4}
$$

$$
= \frac12 \ln(x^2-2x+5) + \arctan\frac{x-1}{2} + C
$$

---

**第4题**  

$$
\int \frac{dx}{x(x^2+1)}
$$
解：  
设

$$
\frac{1}{x(x^2+1)} = \frac{A}{x} + \frac{Bx+C}{x^2+1}
$$

解得 $A=1,\ B=-1,\ C=0$。  
于是

$$
\int \frac{dx}{x(x^2+1)} = \int \left( \frac{1}{x} - \frac{x}{x^2+1} \right) dx
$$

$$
= \ln|x| - \frac12 \ln(x^2+1) + C
$$

---

**第5题**  

$$
\int \frac{3}{x^3+1} dx
$$
解：  
因式分解：$x^3+1 = (x+1)(x^2-x+1)$。  
设

$$
\frac{3}{x^3+1} = \frac{A}{x+1} + \frac{Bx+C}{x^2-x+1}
$$
解得 $A=1,\ B=-1,\ C=2$。  
于是

$$
\int \frac{3}{x^3+1} dx = \int \left( \frac{1}{x+1} + \frac{-x+2}{x^2-x+1} \right) dx
$$

$$
= \ln|x+1| - \frac12 \ln(x^2-x+1) + \sqrt{3}\arctan\frac{2x-1}{\sqrt{3}} + C
$$

---

**第6题** 

$$
\int \frac{x^2+1}{(x+1)^2(x-1)} dx
$$
解：  
设

$$
\frac{x^2+1}{(x+1)^2(x-1)} = \frac{A}{x-1} + \frac{B}{x+1} + \frac{C}{(x+1)^2}
$$
解得 $A=\frac12,\ B=\frac12,\ C=1$。  
于是

$$
\int \frac{x^2+1}{(x+1)^2(x-1)} dx = \frac12 \ln|x-1| + \frac12 \ln|x+1| - \frac{1}{x+1} + C
$$

$$
= \frac12 \ln|x^2-1| - \frac{1}{x+1} + C
$$

---

**第7题**  

$$
\int \frac{x dx}{(x+1)(x+2)(x+3)}
$$
解：  
设

$$
\frac{x}{(x+1)(x+2)(x+3)} = \frac{A}{x+1} + \frac{B}{x+2} + \frac{C}{x+3}
$$
解得 $A=-\frac12,\ B=2,\ C=-\frac32$。  
于是

$$
\int \frac{x dx}{(x+1)(x+2)(x+3)} = -\frac12 \ln|x+1| + 2\ln|x+2| - \frac32 \ln|x+3| + C
$$

---

**第8题**  

$$
\int \frac{x^5+x^4-8}{x^3-x} dx
$$
解：  
多项式除法得：

$$
\frac{x^5+x^4-8}{x^3-x} = x^2+x+1 + \frac{x^2+x-8}{x(x-1)(x+1)}
$$
对分式分解：

$$
\frac{x^2+x-8}{x(x-1)(x+1)} = \frac{A}{x} + \frac{B}{x-1} + \frac{C}{x+1}
$$
解得 $A=8,\ B=-3,\ C=-4$。  
于是

$$
\int \frac{x^5+x^4-8}{x^3-x} dx = \frac13 x^3 + \frac12 x^2 + x + 8\ln|x| - 3\ln|x-1| - 4\ln|x+1| + C
$$

---

**第9题**  

$$
\int \frac{dx}{(x^2+1)(x^2+x)}
$$
解：  
设

$$
\frac{1}{(x^2+1)(x^2+x)} = \frac{A}{x} + \frac{B}{x+1} + \frac{Cx+D}{x^2+1}
$$
解得 $A=1,\ B=-\frac12,\ C=-\frac12,\ D=-\frac12$。  
于是

$$
\int \frac{dx}{(x^2+1)(x^2+x)} = \ln|x| - \frac12 \ln|x+1| - \frac14 \ln(x^2+1) - \frac12 \arctan x + C
$$

---

**第10题**  

$$
\int \frac{1}{x^4-1} dx
$$
解：  
因式分解：$x^4-1 = (x-1)(x+1)(x^2+1)$。  
设

$$
\frac{1}{x^4-1} = \frac{A}{x-1} + \frac{B}{x+1} + \frac{Cx+D}{x^2+1}
$$
解得 $A=\frac14,\ B=-\frac14,\ C=0,\ D=-\frac12$。  
于是

$$
\int \frac{1}{x^4-1} dx = \frac14 \ln|x-1| - \frac14 \ln|x+1| - \frac12 \arctan x + C
$$

---

**第11题** 

$$
\int \frac{dx}{(x^2+1)(x^2+x+1)}
$$
解：  
设

$$
\frac{1}{(x^2+1)(x^2+x+1)} = \frac{Ax+B}{x^2+1} + \frac{Cx+D}{x^2+x+1}
$$
解得 $A=0,\ B=1,\ C=0,\ D=-1$。  
于是

$$
\int \frac{dx}{(x^2+1)(x^2+x+1)} = \arctan x - \frac{2}{\sqrt{3}} \arctan\frac{2x+1}{\sqrt{3}} + C
$$

---

**第12题**  

$$
\int \frac{(x+1)^2}{(x^2+1)^2} dx
$$
解：  
拆项：

$$
\frac{(x+1)^2}{(x^2+1)^2} = \frac{x^2+1}{(x^2+1)^2} + \frac{2x}{(x^2+1)^2} = \frac{1}{x^2+1} + \frac{2x}{(x^2+1)^2}
$$
于是

$$
\int \frac{(x+1)^2}{(x^2+1)^2} dx = \arctan x - \frac{1}{x^2+1} + C
$$

---

**第13题**  

$$
\int \frac{-x^2-2}{(x^2+x+1)^2} dx
$$
解：  
分子拆为：$-x^2-2 = -(x^2+x+1) - (x+1)$。  
于是

$$
\frac{-x^2-2}{(x^2+x+1)^2} = -\frac{1}{x^2+x+1} - \frac{x+1}{(x^2+x+1)^2}
$$
积分得：

$$
\int \frac{-x^2-2}{(x^2+x+1)^2} dx = -\frac{2}{\sqrt{3}} \arctan\frac{2x+1}{\sqrt{3}} + \frac{x}{x^2+x+1} + C
$$

---

**第14题**  

$$
\int \frac{dx}{3+\sin^2 x}
$$
解：  
用恒等式 $\sin^2 x = \frac{1-\cos 2x}{2}$，则

$$
3+\sin^2 x = \frac{7-\cos 2x}{2}
$$
于是原积分 $= 2\int \frac{dx}{7-\cos 2x}$。  
令 $u=2x$，再令 $t=\tan\frac{u}{2}$，可得：

$$
\int \frac{dx}{3+\sin^2 x} = \frac{1}{2\sqrt{3}} \arctan\frac{2\tan x}{\sqrt{3}} + C
$$

---

**第15题**  

$$
\int \frac{dx}{3+\cos x}
$$
解：  
令 $t = \tan\frac{x}{2}$，则

$$
\int \frac{dx}{3+\cos x} = \frac{1}{\sqrt{2}} \arctan\frac{\tan\frac{x}{2}}{\sqrt{2}} + C
$$

---

**第16题**  

$$
\int \frac{dx}{2+\sin x}
$$
解：  
令 $t = \tan\frac{x}{2}$，则

$$
\int \frac{dx}{2+\sin x} = \frac{2}{\sqrt{3}} \arctan\frac{2\tan\frac{x}{2}+1}{\sqrt{3}} + C
$$

---

**第17题**  

$$
\int \frac{dx}{1+\sin x+\cos x}
$$
解：  
令 $t = \tan\frac{x}{2}$，则

$$
\int \frac{dx}{1+\sin x+\cos x} = \ln\left| 1 + \tan\frac{x}{2} \right| + C
$$

---

**第18题**  

$$
\int \frac{dx}{2\sin x-\cos x+5}
$$
解：  
令 $t = \tan\frac{x}{2}$，则

$$
\int \frac{dx}{2\sin x-\cos x+5} = \frac{1}{\sqrt{5}} \arctan\frac{3\tan\frac{x}{2}+1}{\sqrt{5}} + C
$$

---

**第19题**  

$$
\int \frac{dx}{1+\sqrt[3]{x+1}}
$$
解：  
令 $t = \sqrt[3]{x+1}，则 x = t^3-1,\ dx = 3t^2 dt$。  
于是

$$
\int \frac{dx}{1+\sqrt[3]{x+1}} = \int \frac{3t^2}{1+t} dt = 3\int \left( t-1+\frac{1}{1+t} \right) dt
$$

$$
= \frac{3}{2}t^2 - 3t + 3\ln|1+t| + C
$$

$$
= \frac{3}{2}(x+1)^{2/3} - 3(x+1)^{1/3} + 3\ln|1+\sqrt[3]{x+1}| + C
$$

---

**第20题**  

$$
\int \frac{(\sqrt{x})^3-1}{\sqrt{x}+1} dx
$$
解：  
令 $t = \sqrt{x}，则 x = t^2,\ dx = 2t dt$。  
于是

$$
\int \frac{t^3-1}{t+1} \cdot 2t dt = 2\int \frac{t^4 - t}{t+1} dt = 2\int \left( t^3 - t^2 + t - 2 + \frac{2}{t+1} \right) dt
$$

$$
= 2\left( \frac14 t^4 - \frac13 t^3 + \frac12 t^2 - 2t + 2\ln|t+1| \right) + C
$$

$$
= \frac12 x^2 - \frac{2}{3}x^{3/2} + x - 4\sqrt{x} + 4\ln(\sqrt{x}+1) + C
$$

---

**第21题**  

$$
\int \frac{\sqrt{x+1}-1}{\sqrt{x+1}+1} dx
$$
解：  
令 $t = \sqrt{x+1}，则 x = t^2-1,\ dx = 2t dt$。  
于是

$$
\int \frac{t-1}{t+1} \cdot 2t dt = 2\int \frac{t^2 - t}{t+1} dt = 2\int \left( t-2+\frac{2}{t+1} \right) dt
$$

$$
= 2\left( \frac12 t^2 - 2t + 2\ln|t+1| \right) + C
$$

$$
= t^2 - 4t + 4\ln|t+1| + C
$$

$$
= x - 4\sqrt{x+1} + 4\ln(\sqrt{x+1}+1) + C
$$

---

**第22题**  

$$
\int \frac{dx}{\sqrt{x}+\sqrt[4]{x}}
$$
解：  
令 $t = \sqrt[4]{x}，则 x = t^4,\ dx = 4t^3 dt$。  
于是

$$
\int \frac{4t^3}{t^2 + t} dt = 4\int \frac{t^2}{t+1} dt = 4\int \left( t-1+\frac{1}{t+1} \right) dt
$$

$$
= 4\left( \frac12 t^2 - t + \ln|t+1| \right) + C
$$

$$
= 2t^2 - 4t + 4\ln|t+1| + C
$$

$$
= 2\sqrt{x} - 4\sqrt[4]{x} + 4\ln(\sqrt[4]{x}+1) + C
$$

---

**第23题** 

$$\int \sqrt{\frac{1-x}{1+x}} \, \frac{dx}{x}$$


**解**：令  $t = \sqrt{\frac{1-x}{1+x}} \quad \Rightarrow \quad t^2 = \frac{1-x}{1+x}$，解得  $x = \frac{1-t^2}{1+t^2}, \quad dx = \frac{-4t}{(1+t^2)^2} \, dt.$
被积函数化为  

$$\sqrt{\frac{1-x}{1+x}} \cdot \frac{1}{x} \, dx
= t \cdot \frac{1+t^2}{1-t^2} \cdot \frac{-4t}{(1+t^2)^2} \, dt
= \frac{-4t^2}{(1-t^2)(1+t^2)} \, dt.
$$ 

$$I = -\int \left( \frac{2}{1-t^2} - \frac{2}{1+t^2} \right) dt
= 2 \int \frac{dt}{1+t^2} - 2 \int \frac{dt}{1-t^2}.$$

故  

$$I = 2 \arctan t - \ln\left| \frac{1+t}{1-t} \right| + C.$$

回代 ，得  

$$2 \arctan \sqrt{\frac{1-x}{1+x}} - \ln\left| \frac{1+\sqrt{\frac{1-x}{1+x}}}{1-\sqrt{\frac{1-x}{1+x}}} \right| + C.$$

---

**第24题**  

$$
\int \frac{dx}{\sqrt[3]{(x+1)^2(x-1)^4}}
$$
解：  
被积函数为 $(x-1)^{-4/3}(x+1)^{-2/3}$。  
令 $t = \sqrt[3]{\frac{x+1}{x-1}}，则 t^3 = \frac{x+1}{x-1}，得 x = \frac{t^3+1}{t^3-1},\ dx = -\frac{6t^2}{(t^3-1)^2} dt$。  
同时

$$
(x-1)^{-4/3}(x+1)^{-2/3} = \frac{(t^3-1)^2}{4t^2}
$$
于是

$$
\int \frac{dx}{\sqrt[3]{(x+1)^2(x-1)^4}} = \int \frac{(t^3-1)^2}{4t^2} \cdot \left( -\frac{6t^2}{(t^3-1)^2} \right) dt
$$

$$
= -\frac{3}{2} \int dt = -\frac{3}{2} t + C
$$

$$
= -\frac{3}{2} \sqrt[3]{\frac{x+1}{x-1}} + C
$$

---

